<h2 align = "center">
                 Chapter1

####  1.7

![img](https://img-blog.csdnimg.cn/img_convert/90b9153d9218d1821081cb4b11905cd9.png)

![img](https://img-blog.csdnimg.cn/img_convert/3ea00d61ad683aa969d2c765e6f1937a.png)![26629b0c96e30d69284798873797820f.png](https://img-blog.csdnimg.cn/img_convert/26629b0c96e30d69284798873797820f.png)

![e2ca613287a9d22b1579197263819167.png](https://img-blog.csdnimg.cn/img_convert/e2ca613287a9d22b1579197263819167.png)

![26a84b714fb046bc422ea026dd701c82.png](https://img-blog.csdnimg.cn/img_convert/26a84b714fb046bc422ea026dd701c82.png)

![a87df9daf46f35275778e41ecfc9ceb6.png](https://img-blog.csdnimg.cn/img_convert/a87df9daf46f35275778e41ecfc9ceb6.png)

####  1.9

(a) 

$\int_{-\infty}^\infty \vert \Psi(x,t)\vert ^2dx = \int_{-\infty}^\infty A^2e^{-2a\frac{mx^2}{\hbar}}dx = A^2\dfrac{\sqrt{\hbar\pi}}{2\sqrt{2am}} = 1 $

$A = \sqrt[4]{\dfrac{8am}{\hbar\pi}}$

(b)

$\dfrac{\partial \Psi}{\partial t} = \dfrac{i\hbar}{2m}\dfrac{\partial ^2\Psi}{\partial x^2}-\dfrac{i}{\hbar}V\Psi$

$\dfrac{\partial \Psi}{\partial t} = -ai\Psi$

$\dfrac{\partial \Psi}{\partial x} = -\dfrac{2amx}{\hbar}\Psi$

$\dfrac{\partial ^2\Psi}{\partial x^2} = \left(-\dfrac{2am}{\hbar}+\dfrac{4a^2m^2x^2}{\hbar^2}\right)\Psi$

$V = 2a^2mx^2$

(c)

$\langle x\rangle = \int_{-\infty}^\infty x\vert \Psi(x,t)\vert^2dx = \int_{-\infty}^\infty A^2xe^{-2a\frac{mx^2}{\hbar}}dx = 0$

$\langle x^2\rangle = \int_{-\infty}^\infty x^2\vert \Psi(x,t)\vert^2dx = \int_{-\infty}^\infty A^2x^2e^{-2a\frac{mx^2}{\hbar}}dx =\dfrac{\sqrt{\hbar}}{\sqrt{8am}}$

$\langle p\rangle = \dfrac{md\langle x\rangle}{dt} = 0$

$\langle p^2\rangle = \int_{-\infty}^\infty \Psi^*(\dfrac{\hbar}{i}\dfrac{\partial \Psi}{\partial x})^2 \Psi dx = -\hbar^2\int_{-\infty}^\infty\left(-\dfrac{2am}{\hbar}+\dfrac{4a^2m^2x^2}{\hbar^2} \right) \vert \Psi\vert^2 dx $

$= 2am\hbar - \sqrt{2a^3m^3\hbar}$

(d)

$\sigma_x = \sqrt{\langle x^2\rangle -\langle x\rangle^2} = \sqrt[4]{\dfrac{\hbar}{8am}}$

$\sigma_p = \sqrt{\langle p^2\rangle -\langle p\rangle^2} = \sqrt{2am\hbar - \sqrt{2a^3m^3\hbar}}$

$\sigma_x\sigma_p \ge \dfrac{\hbar}{2} $

